src/basic/options.fs
@@ -134,7 +134,7 @@ let specs () : list<Getopt.opt> =
      ( noshort, "print_effect_args", ZeroArgs (fun () -> print_effect_args := true), "Print inferred predicate transformers for all computation types");
      ( noshort, "dump_module", OneArg ((fun x -> dump_module := Some x), "module name"), "");
      ( noshort, "z3timeout", OneArg ((fun s -> z3timeout := Some s), "t"), "Set the Z3 soft timeout to t milliseconds");
-     ( noshort, "logQueries", ZeroArgs (fun () -> logQueries := true), "Log the Z3 queries in $FSTAR_HOME/bin/queries/, or in odir, if set; also see --prn");
+     ( noshort, "logQueries", ZeroArgs (fun () -> logQueries := true), "Log the Z3 queries in queries.smt2");
      ( noshort, "UNSAFE", ZeroArgs (fun () -> Util.print_string "UNSAFE MODE!\n"; __unsafe := true), "");
      ( noshort, "describe_queries", ZeroArgs (fun () -> describe_queries := true), "Print the queried formula and its location");
      ( noshort, "UNSAFE_skip_first_queries", OneArg ((fun x -> skip_first_queries x), "n"), "Skip the first n queries");
