examples/unit-tests/unit1.fst
@@ -97,41 +97,13 @@ val hd_pure: l:list 'a{b2t (is_Cons l)} -> Tot 'a
 let hd_pure l = match l with
   | x::_ -> x
 
+val hd_pure_alt: x:list 'a{b2t (is_Cons x)} -> Tot 'a
+let hd_pure_alt = function
+  | hd::_ -> hd
+
 val dup_pure: x:'a -> Tot ('a * 'a)
 let dup_pure x = (x,x)
 
 val dup_pure_eq: x:'a -> Pure ('a * 'a) True (fun y => MkTuple2._1 y==MkTuple2._2 y)
 let dup_pure_eq x = (x,x)
-
-(* val test_st : m:mode -> State unit *)
-(*                             (fun 'p h0 => (forall h1. SelHeap h1 moderef==SelHeap h0 moderef ==> 'p () h1)) *)
-(* let test_st (m:mode) = *)
-(*   let cur = rd "hello" in *)
-(*   let z = f 0 in *)
-(*   ST.write moderef cur *)
-
-
-(* val test_match: m:mode *)
-(*              -> Wys unit (Requires (fun cur => (if cur.p_or_s==Sec then cur.prins==m.prins else Subset cur.prins m.prins))) *)
-(*                          (Ensures _ (fun m1 a m2 => True)) *)
-(* let test_match (m:mode) = *)
-(*   let cur = get_mode () in *)
-(*   (match cur.p_or_s with *)
-(*    | Sec -> assert (cur.prins == m.prins) *)
-(*    | _ -> assert (Subset cur.prins m.prins)) *)
-
-
-(* val mem: x:'a -> l:list 'a -> bool *)
-(* let rec mem x l = match l with *)
-(*   | [] -> false *)
-(*   | hd::tl -> x=hd || mem x tl *)
-
-(* val hd: x:list 'a{b2t (is_Cons x)} -> Tot 'a *)
-(* let hd = function *)
-(*   | hd::_ -> hd *)
-
-
-
-    
-    
 
