lib/prims.fst
@@ -42,12 +42,16 @@ monad_lattice { (* The definition of the PURE effect is fixed; no user should ev
              kind Post ('a:Type) = 'a => Type
              kind WP ('a:Type) = Post 'a => Pre
              type return ('a:Type) (x:'a) ('p:Post 'a) = 'p x
-             type bind_wp  ('a:Type) ('b:Type) ('wp1:WP 'a) ('wlp1:WP 'a) ('wp2: 'a => WP 'b) ('wlp2:'a => WP 'b) ('p:Post 'b) = 'wp1 (fun a => 'wp2 a 'p)
-             type bind_wlp ('a:Type) ('b:Type) ('wlp1:WP 'a) ('wlp2:'a => WP 'b) ('p:Post 'b) = 'wlp1 (fun a => 'wlp2 a 'p)
+             type bind_wp  ('a:Type) ('b:Type) ('wp1:WP 'a) ('wlp1:WP 'a) 
+                                               ('wp2: 'a => WP 'b) ('wlp2:'a => WP 'b) 
+                                               ('p:Post 'b) = 'wp1 (fun a => 'wp2 a 'p)
+             type bind_wlp ('a:Type) ('b:Type) ('wlp1:WP 'a) 
+                                               ('wlp2:'a => WP 'b) 
+                                               ('p:Post 'b) = 'wlp1 (fun a => 'wlp2 a 'p)
              type ite_wlp ('a:Type) ('wlp_cases:WP 'a) ('post:Post 'a) =
-                 (forall (a:'a). 'wlp_cases (fun a1 => a=!=a1) ==> 'post a)
+                 (forall (a:'a). 'wlp_cases (fun a' => a=!=a') \/ 'post a)
              type ite_wp ('a:Type) ('wlp_cases:WP 'a) ('wp_cases:WP 'a) ('post:Post 'a) =
-                 (forall (a:'a). 'wlp_cases (fun a' => a==a') ==> 'post a)
+                 (forall (a:'a). 'wlp_cases (fun a' => a=!=a') \/ 'post a)
                  /\ ('wp_cases (fun a => True))
              type wp_binop ('a:Type) ('wp1:WP 'a) ('op:Type => Type => Type) ('wp2:WP 'a) ('p:Post 'a) =
                  'op ('wp1 'p) ('wp2 'p)
@@ -61,9 +65,9 @@ monad_lattice { (* The definition of the PURE effect is fixed; no user should ev
              with Pure ('a:Type) ('pre:Pre) ('post:Post 'a) =
                  PURE 'a
                    (fun ('p:Post 'a) => 'pre /\ (forall a. 'post a ==> 'p a)) (* WP *)
-                   (fun ('p:Post 'a) => forall a. 'pre /\ 'post a ==> 'p a)           (* WLP *)
+                   (fun ('p:Post 'a) => forall a. 'pre /\ 'post a ==> 'p a)   (* WLP *)
              and Tot ('a:Type) =
-                 PURE 'a (fun 'p => (forall (x:'a). 'p x)) (fun 'p => (exists (x:'a). 'p x))
+                 PURE 'a (fun 'p => (forall (x:'a). 'p x)) (fun 'p => (forall (x:'a). 'p x))
 }
 open Prims.PURE
 assume type bool
@@ -155,9 +159,9 @@ monad_lattice {
                  'wp1 (fun a h1 => 'wp2 a 'p h1) h0
              type bind_wlp ('a:Type) ('b:Type) ('wlp1:WP 'a) ('wlp2:'a => WP 'b) ('p:Post 'b) (h0:heap) = 'wlp1 (fun a => 'wlp2 a 'p) h0
              type ite_wlp  ('a:Type) ('wlp_cases:WP 'a) ('post:Post 'a) (h0:heap) =
-                 (forall (a:'a) (h:heap). 'wlp_cases (fun a1 h1 => a==a1 /\ h==h1) h0 ==> 'post a h)
+                 (forall (a:'a) (h:heap). 'wlp_cases (fun a1 h1 => a=!=a1 /\ h=!=h1) h0 \/ 'post a h)
              type ite_wp ('a:Type) ('wlp_cases:WP 'a) ('wp_cases:WP 'a) ('post:Post 'a) (h0:heap) =
-                 (forall (a:'a) (h:heap). 'wlp_cases (fun a1 h1 => a==a1 /\ h==h1) h0 ==> 'post a h)
+                 (forall (a:'a) (h:heap). 'wlp_cases (fun a1 h1 => a=!=a1 /\ h=!=h1) h0 \/ 'post a h)
                  /\ 'wp_cases (fun a h_ => True) h0
              type wp_binop ('a:Type) ('wp1:WP 'a) ('op:Type => Type => Type) ('wp2:WP 'a) ('p:Post 'a) (h:heap) =
                  'op ('wp1 'p h) ('wp2 'p h)
@@ -172,7 +176,7 @@ monad_lattice {
              and ST ('a:Type) ('pre:Pre) ('post: heap => Post 'a) (mods:refs) =
                  STATE 'a
                    (fun ('p:Post 'a) (h:heap) => 'pre h /\ (forall a h1. ('pre h /\ Modifies mods h h1 /\ 'post h a h1) ==> 'p a h1)) (* WP *)
-                   (fun ('p:Post 'a) (h:heap) => (exists a h1. ('pre h /\ Modifies mods h h1 /\ 'post h a h1) ==> 'p a h1))           (* WLP *)
+                   (fun ('p:Post 'a) (h:heap) => (forall a h1. ('pre h /\ Modifies mods h h1 /\ 'post h a h1) ==> 'p a h1))           (* WLP *)
 ;
   EXN::
              kind Pre  = Type
@@ -191,9 +195,9 @@ monad_lattice {
                                                                     then 'wlp2 (V.v ra1) (fun rb2 => rb2=!=rb)
                                                                     else  ra1 =!= rb))
              type ite_wlp  ('a:Type) ('wlp_cases:WP 'a) ('post:Post 'a) =
-                 (forall (a:result 'a). 'wlp_cases (fun a1 => a==a1) ==> 'post a)
+                 (forall (a:result 'a). 'wlp_cases (fun a1 => a=!=a1) \/ 'post a)
              type ite_wp ('a:Type) ('wlp_cases:WP 'a) ('wp_cases:WP 'a) ('post:Post 'a) =
-                 (forall (a:result 'a). 'wlp_cases (fun a1 => a==a1) ==> 'post a)
+                 (forall (a:result 'a). 'wlp_cases (fun a1 => a=!=a1) \/ 'post a)
                  /\ 'wp_cases (fun ra2 => True)
              type wp_binop ('a:Type) ('wp1:WP 'a) ('op:Type => Type => Type) ('wp2:WP 'a) ('p:Post 'a) =
                  'op ('wp1 'p) ('wp2 'p)
@@ -207,7 +211,7 @@ monad_lattice {
              with Exn ('a:Type) ('pre:Pre) ('post:Post 'a) =
                  EXN 'a
                    (fun 'p => 'pre /\ (forall (r:result 'a). ('pre /\ 'post r) ==> 'p r)) (* WP *)
-                   (fun 'p => (exists (r:result 'a). ('pre /\ 'post r) ==> 'p r))         (* WLP *)
+                   (fun 'p => (forall (r:result 'a). ('pre /\ 'post r) ==> 'p r))         (* WLP *)
  ;
   ALL::
              kind Pre  = heap => Type
@@ -230,9 +234,9 @@ monad_lattice {
                      then 'wlp2 (V.v ra) (fun rb2 h2 => rb==rb2 /\ h==h2) h1
                      else rb==ra /\ h==h1) h0 ==> 'p rb h)
              type ite_wlp  ('a:Type) ('wlp_cases:WP 'a) ('post:Post 'a) (h0:heap) =
-                 (forall (ra:result 'a) (h:heap). 'wlp_cases (fun ra2 h2 => ra==ra2 /\ h==h2) h0 ==> 'post ra h)
+                 (forall (ra:result 'a) (h:heap). 'wlp_cases (fun ra2 h2 => ra=!=ra2 /\ h=!=h2) h0 \/ 'post ra h)
              type ite_wp ('a:Type) ('wlp_cases:WP 'a) ('wp_cases:WP 'a) ('post:Post 'a) (h0:heap) =
-                 (forall (ra:result 'a) (h:heap). 'wlp_cases (fun ra2 h2 => ra==ra2 /\ h==h2) h0 ==> 'post ra h)
+                 (forall (ra:result 'a) (h:heap). 'wlp_cases (fun ra2 h2 => ra=!=ra2 /\ h=!=h2) h0 \/ 'post ra h)
                  /\ 'wp_cases (fun _a _b => True) h0
              type wp_binop ('a:Type) ('wp1:WP 'a) ('op:Type => Type => Type) ('wp2:WP 'a) ('p:Post 'a) (h:heap) =
                  'op ('wp1 'p h) ('wp2 'p h)
@@ -246,10 +250,10 @@ monad_lattice {
              with All ('a:Type) ('pre:Pre) ('post: heap => Post 'a) (mods:refs) =
                  ALL 'a
                    (fun ('p:Post 'a) (h:heap) => 'pre h /\ (forall ra h1. (Modifies mods h h1 /\ 'post h ra h1) ==> 'p ra h1)) (* WP *)
-                   (fun ('p:Post 'a) (h:heap) => exists ra h1. ('pre h /\ Modifies mods h h1 /\ 'post h ra h1) ==> 'p ra h1)             (* WLP *)
+                   (fun ('p:Post 'a) (h:heap) => forall ra h1. ('pre h /\ Modifies mods h h1 /\ 'post h ra h1) ==> 'p ra h1)             (* WLP *)
              and ML ('a:Type) =
                  ALL 'a (fun 'p h0 => forall (a:result 'a) (h:heap). 'p a h) 
-                        (fun 'p h0 => exists (a:result 'a) (h:heap). 'p a h)
+                        (fun 'p h0 => forall (a:result 'a) (h:heap). 'p a h)
 
   with
   PURE  ~> STATE = (fun ('a:Type) ('wp:PURE.WP 'a) ('p:STATE.Post 'a) (h:heap) => 'wp (fun a => 'p a h));
